# Problem

Solve the recurrence ![T(n)=2T(sqrt(n))+1](http://latex.codecogs.com/gif.latex?T%28n%29%3D2T%28%5Csqrt%7Bn%7D%29%2B1) by making a change of variables. Your solution should be asymptotically tight. Do not worry about whether values are integral.

# Solution

![T(n)=2T(sqrt(n))+1](http://latex.codecogs.com/gif.latex?T%28n%29%3D2T%28%5Csqrt%7Bn%7D%29%2B1)<br>
let ![m=log(n)](http://latex.codecogs.com/gif.latex?m%3Dlog%28n%29), ![n=2^m](http://latex.codecogs.com/gif.latex?n%3D2%5Em)<br>
![⇒T(2^m)=2T(2^(m/2))+1](http://latex.codecogs.com/gif.latex?%5CRightarrow%20T%282%5Em%29%3D2T%282%5E%7B%5Cfrac%7Bm%7D%7B2%7D%7D%29%2B1)<br>
let ![S(m)=T(2^m)](http://latex.codecogs.com/gif.latex?S%28m%29%3DT%282%5Em%29)<br>
![⇒S(m)=2S(m/2)+1](http://latex.codecogs.com/gif.latex?%5CRightarrow%20S%28m%29%3D2S%28%5Cfrac%7Bm%7D%7B2%7D%29%2B1)<br>
by master theorem: a=2, b=2, f(n)=1<br>
![S(m)=m^(log2)=m](http://latex.codecogs.com/gif.latex?S%28m%29%3Dm%5E%7Blog2%7D%3Dm)<br>
![⇒S(m)=\Theta(m)](http://latex.codecogs.com/gif.latex?%5CRightarrow%20S%28m%29%3D%5CTheta%28m%29)<br>
![⇒T(2^m)=\Theta(m)](http://latex.codecogs.com/gif.latex?%5CRightarrow%20T%282%5Em%29%3D%5CTheta%28m%29)<br>
![⇒T(n)=\Theta(logn)](http://latex.codecogs.com/gif.latex?%5CRightarrow%20T%28n%29%3D%5CTheta%28logn%29)
